theories/lang/cpp/logic/ptr_pred.v
@@ -1,0 +1,91 @@
+(*
+ * Copyright (C) BedRock Systems Inc. 2020
+ *
+ * SPDX-License-Identifier: LGPL-2.1 WITH BedRock Exception for use over network, see repository root for details.
+ *)
+From iris.proofmode Require Import tactics.
+From bedrock.lang.prelude Require Import base addr.
+From bedrock.lang.bi Require Import prelude observe.
+From bedrock.lang.cpp Require Import ast semantics.
+From bedrock.lang.cpp Require Import pred.
+
+(* Experimental APIs for observation from pointer predicates, to allow you to
+write a bunch of observations at once.
+*)
+
+Section with_cpp.
+  Context `{Σ : cpp_logic} (σ : genv).
+
+  Lemma observe_strict_valid_valid
+    `(Hobs : !Observe (strict_valid_ptr p) P) :
+    Observe (valid_ptr p) P.
+  Proof. by rewrite /Observe Hobs strict_valid_relaxed. Qed.
+
+  Lemma observe_type_ptr_strict_valid
+    `(Hobs : !Observe (type_ptr ty p) P) :
+    Observe (strict_valid_ptr p) P.
+  Proof. by rewrite /Observe Hobs type_ptr_strict_valid. Qed.
+
+  Lemma observe_type_ptr_valid_plus_one
+    `(Hobs : !Observe (type_ptr ty p) P) :
+    Observe (valid_ptr (p .., o_sub σ ty 1)) P.
+  Proof. by rewrite /Observe Hobs type_ptr_valid_plus_one. Qed.
+End with_cpp.
+
+(* Only import when defining representation predicates and associated instances. *)
+Module ptr_pred_helpers.
+  (* Fail #[export] Existing Instances observe_strict_valid_valid. *)
+  #[export] Hint Resolve
+    observe_strict_valid_valid
+    observe_type_ptr_strict_valid
+    observe_type_ptr_valid_plus_one : typeclass_instances.
+End ptr_pred_helpers.
+
+(* Alternative setup. *)
+Module ptr_pred_observe.
+  (* XXX instances of these classes are easier to declare with less overhead, but the classes
+  themselves cause some backtracking. *)
+  Class ObserveStrictValid `{Σ : cpp_logic} P p := {
+    obs_strict_valid :> Observe (strict_valid_ptr p) P;
+    obs_rel_valid :> Observe (valid_ptr p) P
+  }.
+  Hint Mode ObserveStrictValid ! ! ! - : typeclass_instances.
+
+  Class ObserveTypePtr `{Σ : cpp_logic} P p (σ : genv) ty := {
+    obs_type_ptr :> Observe (type_ptr ty p) P;
+    obs_type_ptr_valid_plus_one :> Observe (valid_ptr (p .., o_sub σ ty 1)) P;
+    obs_type_ptr_strict_valid :> ObserveStrictValid P p;
+  }.
+  Hint Mode ObserveTypePtr ! ! ! - - - : typeclass_instances.
+
+  Section with_cpp.
+    Context `{Σ : cpp_logic} (σ : genv).
+
+    Lemma observe_strict_valid_intro
+      `(Hobs : !Observe (strict_valid_ptr p) P) :
+      ObserveStrictValid P p.
+    Proof. split => //. exact /observe_strict_valid_valid. Qed.
+
+    Lemma observe_type_ptr_intro
+      `(Hobs : !Observe (type_ptr ty p) P) :
+      ObserveTypePtr P p σ ty.
+    Proof.
+      split => //.
+      exact /observe_type_ptr_valid_plus_one.
+      apply /observe_strict_valid_intro /observe_type_ptr_strict_valid.
+    Qed.
+
+    Local Instance tptsto_observe_type_ptr ty q p v :
+      ObserveTypePtr (tptsto ty q p v) p σ ty.
+    Proof. apply /observe_type_ptr_intro /tptsto_type_ptr. Qed.
+
+    Local Instance tptsto_strict_valid_ptr ty q p v :
+      Observe (strict_valid_ptr p) (tptsto ty q p v) := _.
+    Local Instance tptsto_valid_ptr : forall ty q p v,
+      Observe (valid_ptr p) (tptsto ty q p v) := _.
+    Local Instance tptsto_valid_ptr_plus_one : forall ty q p v,
+      Observe (valid_ptr (p .., o_sub σ ty 1)) (tptsto ty q p v) := _.
+  End with_cpp.
+
+  #[export] Hint Resolve tptsto_observe_type_ptr : typeclass_instances.
+End ptr_pred_observe.
